Saner naming schemes, more info stored in translation.

formalization/coerce.v
@@ -6,85 +6,78 @@ Require eitt.
 Axiom cheating : forall A : Type, A.
 Definition todo {A} := cheating A.
 
-Inductive context_coercion : Type :=
-  | ctx_id : context_coercion.
+Inductive ctxcoe : Type :=
+  | ctxcoe_identity : ctxcoe.
 
-Inductive type_coercion : Type :=
-  | type_id : type_coercion
-  | type_cong_prod : type_coercion ->
-                     type_coercion ->
-                     type_coercion
-  | type_cong_id : type_coercion ->
-                   term_coercion ->
-                   term_coercion ->
-                   type_coercion
+Inductive tycoe : Type :=
+  | tycoe_identity : tycoe
+  | tycoe_prod : tycoe -> tycoe -> tycoe
+  | tycoe_id : tycoe -> termcoe -> termcoe -> tycoe
 
-with term_coercion : Type :=
-  | term_id : term_coercion
-  | term_reflection : forall (A : type) (u v p : term), term_coercion.
+with termcoe : Type :=
+  | termcoe_identity : termcoe
+  | termcoe_reflection : forall (A : type) (u v p : term), termcoe.
 
 
 (* Computation of inverses of coercions *)
 
-Definition inv_ctx_coe (crc : context_coercion) : context_coercion :=
+Definition inv_ctxcoe (crc : ctxcoe) : ctxcoe :=
   match crc with
-  | ctx_id => ctx_id
+  | ctxcoe_identity => ctxcoe_identity
   end.
 
-Fixpoint inv_term_coe (crtt : term_coercion) : term_coercion :=
+Fixpoint inv_termcoe (crtt : termcoe) : termcoe :=
   match crtt with
-  | term_id => term_id
-  | term_reflection A u v p =>
-    term_reflection A v u (j A u (Id A (var 1) u) (refl A u) v p)
+  | termcoe_identity => termcoe_identity
+  | termcoe_reflection A u v p =>
+    termcoe_reflection A v u (j A u (Id A (var 1) u) (refl A u) v p)
   end.
 
-Fixpoint inv_type_coe (crt : type_coercion) : type_coercion :=
+Fixpoint inv_tycoe (crt : tycoe) : tycoe :=
   match crt with
-  | type_id => type_id
-  | type_cong_prod cA cB => type_cong_prod (inv_type_coe cA) (inv_type_coe cB)
-  | type_cong_id cA cu cv => type_cong_id (inv_type_coe cA)
-                                         (inv_term_coe cu)
-                                         (inv_term_coe cv)
+  | tycoe_identity => tycoe_identity
+  | tycoe_prod cA cB => tycoe_prod (inv_tycoe cA) (inv_tycoe cB)
+  | tycoe_id cA cu cv => tycoe_id (inv_tycoe cA) (inv_termcoe cu) (inv_termcoe cv)
   end.
 
 
 (* Action of coercions on expressions *)
 
-Fixpoint act_subst_left (crc : context_coercion) (sbs : substitution) : substitution :=
+Fixpoint act_subst_left (crc : ctxcoe) (sbs : substitution) : substitution :=
   match crc with
     | ctx_id => sbs
   end.
 
-Fixpoint act_subst_right (crc : context_coercion) (sbs : substitution) : substitution :=
+Fixpoint act_subst_right (crc : ctxcoe) (sbs : substitution) : substitution :=
   match crc with
     | ctx_id => sbs
   end.
 
-Definition act_subst (crc1 crc2 : context_coercion) (sbs : substitution) :=
+Definition act_subst (crc1 crc2 : ctxcoe) (sbs : substitution) :=
   act_subst_left crc1 (act_subst_right crc2 sbs).
 
-Fixpoint act_type (crc : context_coercion) (A : type) :=
+Fixpoint act_type (crc : ctxcoe) (A : type) :=
   match crc with
   | ctx_id => A
   end.
 
-Fixpoint act_term_ctx (crc : context_coercion) (u : term) : term :=
+Fixpoint act_term_ctx (crc : ctxcoe) (u : term) : term :=
   match crc with
   | ctx_id => u
   end.
 
-Fixpoint act_term_type (crc : type_coercion) (u : term) : term :=
+Fixpoint act_term_type (crc : tycoe) (u : term) : term :=
   match crc with
-  | type_id => u
-  | type_cong_prod cA cB => todo (* Problem with the definition of cB! *)
-  | type_cong_id cA cu cv => todo (* I'm a bit lost *)
+  | tycoe_identity => u
+  | tycoe_prod cA cB => todo (* Problem with the definition of cB! *)
+  | tycoe_id cA cu cv => todo (* I'm a bit lost *)
   end.
 
-Definition act_term (crc : context_coercion) (crt : type_coercion) (u : term) : term :=
+Definition act_term (crc : ctxcoe) (crt : tycoe) (u : term) : term :=
   act_term_type crt (act_term_ctx crc u).
 
-Inductive isctxcoe : context_coercion -> context -> context -> Type :=
-  | isctx_id : forall G, eitt.isctx G -> isctxcoe ctx_id G G.
+Inductive isctxcoe : ctxcoe -> context -> context -> Type :=
+  | isctxcoe_identity : forall G, eitt.isctx G -> isctxcoe ctxcoe_identity G G.
 
-Inductive istypecoe : type_coercion -> type -> type -> Type :=
-  | istype_id : forall {G A B}, eitt.eqtype G A B -> istypecoe type_id A B.
+Inductive istypecoe : tycoe -> type -> type -> Type :=
+  | istycoe_identity : forall {G A B}, eitt.eqtype G A B -> istypecoe tycoe_identity A B.
